Compose staged protected replay witnesses
Co-authored-by: Copilot <223556219+Copilot@users.noreply.github.com>

src/spec/TLS13.ConnectionState.ProtectedWireLemmas.fst
@@ -8771,6 +8771,565 @@ let lemma_protected_handshake_event_projection_pair_after_client_finished_local_
               server_tail_sent
               server_tail_received
             and () ) ) ) ) )
+#push-options "--split_queries always --z3rlimit 10"
+let lemma_paired_protected_handshake_event_projection_pair_witnesses_from_staged_replays
+  (client_state:connection_state)
+  (server_state:connection_state)
+  (server_flight_sender:connection_model)
+  (server_flight_receiver:connection_model)
+  (server_after_install:connection_model)
+  (client_after_install:connection_model)
+  (server_after0:connection_model)
+  (client_after0:connection_model)
+  (server_after1:connection_model)
+  (client_after1:connection_model)
+  (server_after_auth_skip:connection_model)
+  (client_after_auth_skip:connection_model)
+  (server_after2:connection_model)
+  (client_after2:connection_model)
+  (client_after_verify_skip:connection_model)
+  (server_after3:connection_model)
+  (client_after3:connection_model)
+  (server_auth_skip:local_event)
+  (client_auth_skip:local_event)
+  (client_verify_skip:local_event)
+  (server_material:traffic_key_material)
+  (client_material:traffic_key_material)
+  (sent_msg0:M.handshake_msg)
+  (received_msg0:M.handshake_msg)
+  (sent_msg1:M.handshake_msg)
+  (received_msg1:M.handshake_msg)
+  (sent_msg2:M.handshake_msg)
+  (received_msg2:M.handshake_msg)
+  (sent_msg3:M.handshake_msg)
+  (received_msg3:M.handshake_msg)
+  (server_rest:list conn_event)
+  (client_rest:list conn_event)
+  (server_raw_sent:B.bytes)
+  (server_raw_received:B.bytes)
+  (client_raw_sent:B.bytes)
+  (client_raw_received:B.bytes)
+  (server_final:connection_model)
+  (client_final:connection_model)
+  (client_finished_sender:connection_model)
+  (client_finished_receiver:connection_model)
+  (cf_client_after_verify:connection_model)
+  (cf_client_after_app_write:connection_model)
+  (cf_client_after_app_read:connection_model)
+  (cf_server_after_app_write:connection_model)
+  (cf_client_after_finished:connection_model)
+  (cf_server_after_finished:connection_model)
+  (verified_server_finished:M.finished)
+  (client_app_write_material:traffic_key_material)
+  (client_app_read_material:traffic_key_material)
+  (server_app_write_material:traffic_key_material)
+  (sent_msg4:M.handshake_msg)
+  (received_msg4:M.handshake_msg)
+  (client_finished_rest:list conn_event)
+  (server_finished_rest:list conn_event)
+  (client_finished_raw_sent:B.bytes)
+  (client_finished_raw_received:B.bytes)
+  (server_finished_raw_sent:B.bytes)
+  (server_finished_raw_received:B.bytes)
+  (client_finished_final:connection_model)
+  (server_finished_final:connection_model)
+  : Lemma
+      (requires
+        (match
+          client_state.cs_model.model_handshake.hs_encrypted_extensions,
+          server_state.cs_model.model_handshake.hs_encrypted_extensions,
+          client_state.cs_model.model_handshake.hs_certificate,
+          server_state.cs_model.model_handshake.hs_certificate,
+          client_state.cs_model.model_handshake.hs_certificate_verify,
+          server_state.cs_model.model_handshake.hs_certificate_verify,
+          client_state.cs_model.model_handshake.hs_server_finished,
+          server_state.cs_model.model_handshake.hs_server_finished,
+          client_state.cs_model.model_handshake.hs_client_finished,
+          server_state.cs_model.model_handshake.hs_client_finished
+        with
+        | Some client_ee, Some server_ee_msg,
+          Some client_cert, Some server_cert_msg,
+          Some client_cv, Some server_cv_msg,
+          Some client_sf, Some server_sf,
+          Some client_cf, Some server_cf ->
+          sent_msg0 == M.EncryptedExtensions server_ee_msg /\
+          received_msg0 == M.EncryptedExtensions client_ee /\
+          sent_msg1 == M.Certificate server_cert_msg /\
+          received_msg1 == M.Certificate client_cert /\
+          sent_msg2 == M.CertificateVerify server_cv_msg /\
+          received_msg2 == M.CertificateVerify client_cv /\
+          sent_msg3 == M.Finished server_sf /\
+          received_msg3 == M.Finished client_sf /\
+          sent_msg4 == M.Finished client_cf /\
+          received_msg4 == M.Finished server_cf
+        | _, _, _, _, _, _, _, _, _, _ ->
+          False) /\
+        (match
+          server_flight_sender.model_handshake.hs_keys.ks_handshake_secret,
+          server_flight_receiver.model_handshake.hs_keys.ks_handshake_secret
+        with
+        | Some server_secret, Some client_secret ->
+          Seq.equal server_secret client_secret
+        | _, _ ->
+          False) /\
+        Seq.equal
+          server_flight_sender.model_handshake.hs_transcript
+          server_flight_receiver.model_handshake.hs_transcript /\
+        local_event_does_not_install_record_keys server_auth_skip /\
+        local_event_does_not_install_record_keys client_auth_skip /\
+        local_event_does_not_install_record_keys client_verify_skip /\
+        Seq.equal server_raw_sent client_raw_received /\
+        protected_handshake_wire_round_trip_message sent_msg0 /\
+        protected_handshake_wire_round_trip_message received_msg0 /\
+        protected_handshake_wire_round_trip_message sent_msg1 /\
+        protected_handshake_wire_round_trip_message received_msg1 /\
+        protected_handshake_wire_round_trip_message sent_msg2 /\
+        protected_handshake_wire_round_trip_message received_msg2 /\
+        protected_handshake_wire_round_trip_message sent_msg3 /\
+        protected_handshake_wire_round_trip_message received_msg3 /\
+        step_model
+          server_flight_sender
+          (ConnLocalEvent
+            (LocalInstallTrafficKeysForRole {
+              install_role = ServerEndpoint;
+              install_payload = {
+                install_epoch = TrafficHandshake;
+                install_direction = TrafficWrite;
+                install_material = server_material;
+              };
+            })) == Some server_after_install /\
+        step_model
+          server_flight_receiver
+          (ConnLocalEvent
+            (LocalInstallTrafficKeys {
+              install_epoch = TrafficHandshake;
+              install_direction = TrafficRead;
+              install_material = client_material;
+            })) == Some client_after_install /\
+        step_model
+          server_after_install
+          (ConnNetworkEvent {
+            CL.message_direction = CL.Sent;
+            CL.message_value = M.TlsHandshake sent_msg0;
+          }) == Some server_after0 /\
+        step_model
+          client_after_install
+          (ConnNetworkEvent {
+            CL.message_direction = CL.Received;
+            CL.message_value = M.TlsHandshake received_msg0;
+          }) == Some client_after0 /\
+        server_after0.model_record.record_write ==
+          R.next_seq server_after_install.model_record.record_write /\
+        client_after0.model_record.record_read ==
+          R.next_seq client_after_install.model_record.record_read /\
+        step_model
+          server_after0
+          (ConnNetworkEvent {
+            CL.message_direction = CL.Sent;
+            CL.message_value = M.TlsHandshake sent_msg1;
+          }) == Some server_after1 /\
+        step_model
+          client_after0
+          (ConnNetworkEvent {
+            CL.message_direction = CL.Received;
+            CL.message_value = M.TlsHandshake received_msg1;
+          }) == Some client_after1 /\
+        server_after1.model_record.record_write ==
+          R.next_seq server_after0.model_record.record_write /\
+        client_after1.model_record.record_read ==
+          R.next_seq client_after0.model_record.record_read /\
+        step_model server_after1 (ConnLocalEvent server_auth_skip) ==
+          Some server_after_auth_skip /\
+        step_model client_after1 (ConnLocalEvent client_auth_skip) ==
+          Some client_after_auth_skip /\
+        step_model
+          server_after_auth_skip
+          (ConnNetworkEvent {
+            CL.message_direction = CL.Sent;
+            CL.message_value = M.TlsHandshake sent_msg2;
+          }) == Some server_after2 /\
+        step_model
+          client_after_auth_skip
+          (ConnNetworkEvent {
+            CL.message_direction = CL.Received;
+            CL.message_value = M.TlsHandshake received_msg2;
+          }) == Some client_after2 /\
+        server_after2.model_record.record_write ==
+          R.next_seq server_after_auth_skip.model_record.record_write /\
+        client_after2.model_record.record_read ==
+          R.next_seq client_after_auth_skip.model_record.record_read /\
+        step_model client_after2 (ConnLocalEvent client_verify_skip) ==
+          Some client_after_verify_skip /\
+        step_model
+          server_after2
+          (ConnNetworkEvent {
+            CL.message_direction = CL.Sent;
+            CL.message_value = M.TlsHandshake sent_msg3;
+          }) == Some server_after3 /\
+        step_model
+          client_after_verify_skip
+          (ConnNetworkEvent {
+            CL.message_direction = CL.Received;
+            CL.message_value = M.TlsHandshake received_msg3;
+          }) == Some client_after3 /\
+        server_after3.model_record.record_write ==
+          R.next_seq server_after2.model_record.record_write /\
+        client_after3.model_record.record_read ==
+          R.next_seq client_after_verify_skip.model_record.record_read /\
+        conn_events_sent_seal_replay
+          server_flight_sender
+          (ConnLocalEvent
+            (LocalInstallTrafficKeysForRole {
+              install_role = ServerEndpoint;
+              install_payload = {
+                install_epoch = TrafficHandshake;
+                install_direction = TrafficWrite;
+                install_material = server_material;
+              };
+            }) :: ConnNetworkEvent {
+              CL.message_direction = CL.Sent;
+              CL.message_value = M.TlsHandshake sent_msg0;
+            } :: ConnNetworkEvent {
+              CL.message_direction = CL.Sent;
+              CL.message_value = M.TlsHandshake sent_msg1;
+            } :: ConnLocalEvent server_auth_skip :: ConnNetworkEvent {
+              CL.message_direction = CL.Sent;
+              CL.message_value = M.TlsHandshake sent_msg2;
+            } :: ConnNetworkEvent {
+              CL.message_direction = CL.Sent;
+              CL.message_value = M.TlsHandshake sent_msg3;
+            } :: server_rest)
+          server_raw_sent
+          server_raw_received
+          server_final /\
+        conn_events_received_decode_replay
+          server_flight_receiver
+          (ConnLocalEvent
+            (LocalInstallTrafficKeys {
+              install_epoch = TrafficHandshake;
+              install_direction = TrafficRead;
+              install_material = client_material;
+            }) :: ConnNetworkEvent {
+              CL.message_direction = CL.Received;
+              CL.message_value = M.TlsHandshake received_msg0;
+            } :: ConnNetworkEvent {
+              CL.message_direction = CL.Received;
+              CL.message_value = M.TlsHandshake received_msg1;
+            } :: ConnLocalEvent client_auth_skip :: ConnNetworkEvent {
+              CL.message_direction = CL.Received;
+              CL.message_value = M.TlsHandshake received_msg2;
+            } :: ConnLocalEvent client_verify_skip :: ConnNetworkEvent {
+              CL.message_direction = CL.Received;
+              CL.message_value = M.TlsHandshake received_msg3;
+            } :: client_rest)
+          client_raw_sent
+          client_raw_received
+          client_final /\
+        write_read_record_material_aligned
+          client_finished_sender
+          client_finished_receiver /\
+        Seq.equal client_finished_raw_sent server_finished_raw_received /\
+        protected_handshake_wire_round_trip_message sent_msg4 /\
+        protected_handshake_wire_round_trip_message received_msg4 /\
+        step_model
+          client_finished_sender
+          (ConnLocalEvent (LocalVerifyFinished verified_server_finished)) ==
+          Some cf_client_after_verify /\
+        step_model
+          cf_client_after_verify
+          (ConnLocalEvent
+            (LocalInstallTrafficKeys {
+              install_epoch = TrafficApplication;
+              install_direction = TrafficWrite;
+              install_material = client_app_write_material;
+            })) == Some cf_client_after_app_write /\
+        step_model
+          cf_client_after_app_write
+          (ConnLocalEvent
+            (LocalInstallTrafficKeys {
+              install_epoch = TrafficApplication;
+              install_direction = TrafficRead;
+              install_material = client_app_read_material;
+            })) == Some cf_client_after_app_read /\
+        step_model
+          client_finished_receiver
+          (ConnLocalEvent
+            (LocalInstallTrafficKeysForRole {
+              install_role = ServerEndpoint;
+              install_payload = {
+                install_epoch = TrafficApplication;
+                install_direction = TrafficWrite;
+                install_material = server_app_write_material;
+              };
+            })) == Some cf_server_after_app_write /\
+        step_model
+          cf_client_after_app_read
+          (ConnNetworkEvent {
+            CL.message_direction = CL.Sent;
+            CL.message_value = M.TlsHandshake sent_msg4;
+          }) == Some cf_client_after_finished /\
+        step_model
+          cf_server_after_app_write
+          (ConnNetworkEvent {
+            CL.message_direction = CL.Received;
+            CL.message_value = M.TlsHandshake received_msg4;
+          }) == Some cf_server_after_finished /\
+        conn_events_sent_seal_replay
+          client_finished_sender
+          (ConnLocalEvent (LocalVerifyFinished verified_server_finished) ::
+           ConnLocalEvent
+             (LocalInstallTrafficKeys {
+               install_epoch = TrafficApplication;
+               install_direction = TrafficWrite;
+               install_material = client_app_write_material;
+             }) ::
+           ConnLocalEvent
+             (LocalInstallTrafficKeys {
+               install_epoch = TrafficApplication;
+               install_direction = TrafficRead;
+               install_material = client_app_read_material;
+             }) ::
+           ConnNetworkEvent {
+             CL.message_direction = CL.Sent;
+             CL.message_value = M.TlsHandshake sent_msg4;
+           } :: client_finished_rest)
+          client_finished_raw_sent
+          client_finished_raw_received
+          client_finished_final /\
+        conn_events_received_decode_replay
+          client_finished_receiver
+          (ConnLocalEvent
+             (LocalInstallTrafficKeysForRole {
+               install_role = ServerEndpoint;
+               install_payload = {
+                 install_epoch = TrafficApplication;
+                 install_direction = TrafficWrite;
+                 install_material = server_app_write_material;
+               };
+             }) ::
+           ConnNetworkEvent {
+             CL.message_direction = CL.Received;
+             CL.message_value = M.TlsHandshake received_msg4;
+           } :: server_finished_rest)
+          server_finished_raw_sent
+          server_finished_raw_received
+          server_finished_final)
+      (ensures
+        exists server_ee server_cert server_cv server_finished client_finished.
+          paired_protected_handshake_event_projection_pairs
+            client_state
+            server_state
+            server_ee
+            server_cert
+            server_cv
+            server_finished
+            client_finished)
+=
+  lemma_protected_handshake_event_projection_pairs_after_server_write_client_read_install_server_encrypted_flight_with_tails
+    server_flight_sender
+    server_flight_receiver
+    server_after_install
+    client_after_install
+    server_after0
+    client_after0
+    server_after1
+    client_after1
+    server_after_auth_skip
+    client_after_auth_skip
+    server_after2
+    client_after2
+    client_after_verify_skip
+    server_after3
+    client_after3
+    server_auth_skip
+    client_auth_skip
+    client_verify_skip
+    server_material
+    client_material
+    sent_msg0
+    received_msg0
+    sent_msg1
+    received_msg1
+    sent_msg2
+    received_msg2
+    sent_msg3
+    received_msg3
+    server_rest
+    client_rest
+    server_raw_sent
+    server_raw_received
+    client_raw_sent
+    client_raw_received
+    server_final
+    client_final;
+  eliminate exists
+    (pair0:protected_message_replay)
+    (pair1:protected_message_replay)
+    (pair2:protected_message_replay)
+    (pair3:protected_message_replay)
+    (server_tail_sent:B.bytes)
+    (server_tail_received:B.bytes)
+    (client_tail_sent:B.bytes)
+    (client_tail_received:B.bytes).
+    pair0.pm_sender == server_after_install /\
+    pair0.pm_receiver == client_after_install /\
+    protected_handshake_event_projection_pair
+      pair0
+      sent_msg0
+      received_msg0 /\
+    pair1.pm_sender == server_after0 /\
+    pair1.pm_receiver == client_after0 /\
+    protected_handshake_event_projection_pair
+      pair1
+      sent_msg1
+      received_msg1 /\
+    pair2.pm_sender == server_after_auth_skip /\
+    pair2.pm_receiver == client_after_auth_skip /\
+    protected_handshake_event_projection_pair
+      pair2
+      sent_msg2
+      received_msg2 /\
+    pair3.pm_sender == server_after2 /\
+    pair3.pm_receiver == client_after_verify_skip /\
+    protected_handshake_event_projection_pair
+      pair3
+      sent_msg3
+      received_msg3 /\
+    write_read_record_material_aligned server_after3 client_after3 /\
+    Seq.equal server_tail_sent client_tail_received /\
+    conn_events_sent_seal_replay
+      server_after3
+      server_rest
+      server_tail_sent
+      server_tail_received
+      server_final /\
+    conn_events_received_decode_replay
+      client_after3
+      client_rest
+      client_tail_sent
+      client_tail_received
+      client_final
+  returns
+    exists server_ee server_cert server_cv server_finished client_finished.
+      paired_protected_handshake_event_projection_pairs
+        client_state
+        server_state
+        server_ee
+        server_cert
+        server_cv
+        server_finished
+        client_finished
+  with _.
+  ( lemma_protected_handshake_event_projection_pair_after_client_finished_local_skips_with_tails
+      client_finished_sender
+      client_finished_receiver
+      cf_client_after_verify
+      cf_client_after_app_write
+      cf_client_after_app_read
+      cf_server_after_app_write
+      cf_client_after_finished
+      cf_server_after_finished
+      verified_server_finished
+      client_app_write_material
+      client_app_read_material
+      server_app_write_material
+      sent_msg4
+      received_msg4
+      client_finished_rest
+      server_finished_rest
+      client_finished_raw_sent
+      client_finished_raw_received
+      server_finished_raw_sent
+      server_finished_raw_received
+      client_finished_final
+      server_finished_final;
+    eliminate exists
+      (pair4:protected_message_replay)
+      (cf_client_tail_sent:B.bytes)
+      (cf_client_tail_received:B.bytes)
+      (cf_server_tail_sent:B.bytes)
+      (cf_server_tail_received:B.bytes).
+      pair4.pm_sender == cf_client_after_app_read /\
+      pair4.pm_receiver == cf_server_after_app_write /\
+      protected_handshake_event_projection_pair
+        pair4
+        sent_msg4
+        received_msg4 /\
+      Seq.equal cf_client_tail_sent cf_server_tail_received /\
+      conn_events_sent_seal_replay
+        cf_client_after_finished
+        client_finished_rest
+        cf_client_tail_sent
+        cf_client_tail_received
+        client_finished_final /\
+      conn_events_received_decode_replay
+        cf_server_after_finished
+        server_finished_rest
+        cf_server_tail_sent
+        cf_server_tail_received
+        server_finished_final
+    returns
+      exists server_ee server_cert server_cv server_finished client_finished.
+        paired_protected_handshake_event_projection_pairs
+          client_state
+          server_state
+          server_ee
+          server_cert
+          server_cv
+          server_finished
+          client_finished
+    with _.
+    ( let client_hs = client_state.cs_model.model_handshake in
+      let server_hs = server_state.cs_model.model_handshake in
+      match
+        client_hs.hs_encrypted_extensions,
+        server_hs.hs_encrypted_extensions,
+        client_hs.hs_certificate,
+        server_hs.hs_certificate,
+        client_hs.hs_certificate_verify,
+        server_hs.hs_certificate_verify,
+        client_hs.hs_server_finished,
+        server_hs.hs_server_finished,
+        client_hs.hs_client_finished,
+        server_hs.hs_client_finished
+      with
+      | Some client_ee, Some server_ee_msg,
+        Some client_cert, Some server_cert_msg,
+        Some client_cv, Some server_cv_msg,
+        Some client_sf, Some server_sf,
+        Some client_cf, Some server_cf ->
+        assert (sent_msg0 == M.EncryptedExtensions server_ee_msg);
+        assert (received_msg0 == M.EncryptedExtensions client_ee);
+        assert (sent_msg1 == M.Certificate server_cert_msg);
+        assert (received_msg1 == M.Certificate client_cert);
+        assert (sent_msg2 == M.CertificateVerify server_cv_msg);
+        assert (received_msg2 == M.CertificateVerify client_cv);
+        assert (sent_msg3 == M.Finished server_sf);
+        assert (received_msg3 == M.Finished client_sf);
+        assert (sent_msg4 == M.Finished client_cf);
+        assert (received_msg4 == M.Finished server_cf);
+        lemma_paired_protected_handshake_event_projection_pair_witnesses_intro_from_messages
+          client_state
+          server_state
+          pair0
+          pair1
+          pair2
+          pair3
+          pair4
+          sent_msg0
+          received_msg0
+          sent_msg1
+          received_msg1
+          sent_msg2
+          received_msg2
+          sent_msg3
+          received_msg3
+          sent_msg4
+          received_msg4
+      | _, _, _, _, _, _, _, _, _, _ ->
+        assert False ) )
+#pop-options
+
 #pop-options
 
 let lemma_protected_handshake_event_projection_pair_after_sender_received_network_head
