src/spec/TLS13.ConnectionState.ProtectedWireLemmas.fsti
@@ -3884,6 +3884,359 @@ val lemma_protected_handshake_event_projection_pair_after_client_finished_local_
             server_tail_received
             server_final)
 
+val lemma_paired_protected_handshake_event_projection_pair_witnesses_from_staged_replays
+  (client_state:CS.connection_state)
+  (server_state:CS.connection_state)
+  (server_flight_sender:CS.connection_model)
+  (server_flight_receiver:CS.connection_model)
+  (server_after_install:CS.connection_model)
+  (client_after_install:CS.connection_model)
+  (server_after0:CS.connection_model)
+  (client_after0:CS.connection_model)
+  (server_after1:CS.connection_model)
+  (client_after1:CS.connection_model)
+  (server_after_auth_skip:CS.connection_model)
+  (client_after_auth_skip:CS.connection_model)
+  (server_after2:CS.connection_model)
+  (client_after2:CS.connection_model)
+  (client_after_verify_skip:CS.connection_model)
+  (server_after3:CS.connection_model)
+  (client_after3:CS.connection_model)
+  (server_auth_skip:CS.local_event)
+  (client_auth_skip:CS.local_event)
+  (client_verify_skip:CS.local_event)
+  (server_material:CS.traffic_key_material)
+  (client_material:CS.traffic_key_material)
+  (sent_msg0:M.handshake_msg)
+  (received_msg0:M.handshake_msg)
+  (sent_msg1:M.handshake_msg)
+  (received_msg1:M.handshake_msg)
+  (sent_msg2:M.handshake_msg)
+  (received_msg2:M.handshake_msg)
+  (sent_msg3:M.handshake_msg)
+  (received_msg3:M.handshake_msg)
+  (server_rest:list CS.conn_event)
+  (client_rest:list CS.conn_event)
+  (server_raw_sent:B.bytes)
+  (server_raw_received:B.bytes)
+  (client_raw_sent:B.bytes)
+  (client_raw_received:B.bytes)
+  (server_final:CS.connection_model)
+  (client_final:CS.connection_model)
+  (client_finished_sender:CS.connection_model)
+  (client_finished_receiver:CS.connection_model)
+  (cf_client_after_verify:CS.connection_model)
+  (cf_client_after_app_write:CS.connection_model)
+  (cf_client_after_app_read:CS.connection_model)
+  (cf_server_after_app_write:CS.connection_model)
+  (cf_client_after_finished:CS.connection_model)
+  (cf_server_after_finished:CS.connection_model)
+  (verified_server_finished:M.finished)
+  (client_app_write_material:CS.traffic_key_material)
+  (client_app_read_material:CS.traffic_key_material)
+  (server_app_write_material:CS.traffic_key_material)
+  (sent_msg4:M.handshake_msg)
+  (received_msg4:M.handshake_msg)
+  (client_finished_rest:list CS.conn_event)
+  (server_finished_rest:list CS.conn_event)
+  (client_finished_raw_sent:B.bytes)
+  (client_finished_raw_received:B.bytes)
+  (server_finished_raw_sent:B.bytes)
+  (server_finished_raw_received:B.bytes)
+  (client_finished_final:CS.connection_model)
+  (server_finished_final:CS.connection_model)
+  : Lemma
+      (requires
+        (match
+          client_state.CS.cs_model.CS.model_handshake.CS.hs_encrypted_extensions,
+          server_state.CS.cs_model.CS.model_handshake.CS.hs_encrypted_extensions,
+          client_state.CS.cs_model.CS.model_handshake.CS.hs_certificate,
+          server_state.CS.cs_model.CS.model_handshake.CS.hs_certificate,
+          client_state.CS.cs_model.CS.model_handshake.CS.hs_certificate_verify,
+          server_state.CS.cs_model.CS.model_handshake.CS.hs_certificate_verify,
+          client_state.CS.cs_model.CS.model_handshake.CS.hs_server_finished,
+          server_state.CS.cs_model.CS.model_handshake.CS.hs_server_finished,
+          client_state.CS.cs_model.CS.model_handshake.CS.hs_client_finished,
+          server_state.CS.cs_model.CS.model_handshake.CS.hs_client_finished
+        with
+        | Some client_ee, Some server_ee_msg,
+          Some client_cert, Some server_cert_msg,
+          Some client_cv, Some server_cv_msg,
+          Some client_sf, Some server_sf,
+          Some client_cf, Some server_cf ->
+          sent_msg0 == M.EncryptedExtensions server_ee_msg /\
+          received_msg0 == M.EncryptedExtensions client_ee /\
+          sent_msg1 == M.Certificate server_cert_msg /\
+          received_msg1 == M.Certificate client_cert /\
+          sent_msg2 == M.CertificateVerify server_cv_msg /\
+          received_msg2 == M.CertificateVerify client_cv /\
+          sent_msg3 == M.Finished server_sf /\
+          received_msg3 == M.Finished client_sf /\
+          sent_msg4 == M.Finished client_cf /\
+          received_msg4 == M.Finished server_cf
+        | _, _, _, _, _, _, _, _, _, _ ->
+          False) /\
+        (match
+          server_flight_sender.CS.model_handshake.CS.hs_keys.CS.ks_handshake_secret,
+          server_flight_receiver.CS.model_handshake.CS.hs_keys.CS.ks_handshake_secret
+        with
+        | Some server_secret, Some client_secret ->
+          Seq.equal server_secret client_secret
+        | _, _ ->
+          False) /\
+        Seq.equal
+          server_flight_sender.CS.model_handshake.CS.hs_transcript
+          server_flight_receiver.CS.model_handshake.CS.hs_transcript /\
+        local_event_does_not_install_record_keys server_auth_skip /\
+        local_event_does_not_install_record_keys client_auth_skip /\
+        local_event_does_not_install_record_keys client_verify_skip /\
+        Seq.equal server_raw_sent client_raw_received /\
+        protected_handshake_wire_round_trip_message sent_msg0 /\
+        protected_handshake_wire_round_trip_message received_msg0 /\
+        protected_handshake_wire_round_trip_message sent_msg1 /\
+        protected_handshake_wire_round_trip_message received_msg1 /\
+        protected_handshake_wire_round_trip_message sent_msg2 /\
+        protected_handshake_wire_round_trip_message received_msg2 /\
+        protected_handshake_wire_round_trip_message sent_msg3 /\
+        protected_handshake_wire_round_trip_message received_msg3 /\
+        CS.step_model
+          server_flight_sender
+          (CS.ConnLocalEvent
+            (CS.LocalInstallTrafficKeysForRole {
+              CS.install_role = CS.ServerEndpoint;
+              CS.install_payload = {
+                CS.install_epoch = CS.TrafficHandshake;
+                CS.install_direction = CS.TrafficWrite;
+                CS.install_material = server_material;
+              };
+            })) == Some server_after_install /\
+        CS.step_model
+          server_flight_receiver
+          (CS.ConnLocalEvent
+            (CS.LocalInstallTrafficKeys {
+              CS.install_epoch = CS.TrafficHandshake;
+              CS.install_direction = CS.TrafficRead;
+              CS.install_material = client_material;
+            })) == Some client_after_install /\
+        CS.step_model
+          server_after_install
+          (CS.ConnNetworkEvent {
+            CL.message_direction = CL.Sent;
+            CL.message_value = M.TlsHandshake sent_msg0;
+          }) == Some server_after0 /\
+        CS.step_model
+          client_after_install
+          (CS.ConnNetworkEvent {
+            CL.message_direction = CL.Received;
+            CL.message_value = M.TlsHandshake received_msg0;
+          }) == Some client_after0 /\
+        server_after0.CS.model_record.CS.record_write ==
+          R.next_seq server_after_install.CS.model_record.CS.record_write /\
+        client_after0.CS.model_record.CS.record_read ==
+          R.next_seq client_after_install.CS.model_record.CS.record_read /\
+        CS.step_model
+          server_after0
+          (CS.ConnNetworkEvent {
+            CL.message_direction = CL.Sent;
+            CL.message_value = M.TlsHandshake sent_msg1;
+          }) == Some server_after1 /\
+        CS.step_model
+          client_after0
+          (CS.ConnNetworkEvent {
+            CL.message_direction = CL.Received;
+            CL.message_value = M.TlsHandshake received_msg1;
+          }) == Some client_after1 /\
+        server_after1.CS.model_record.CS.record_write ==
+          R.next_seq server_after0.CS.model_record.CS.record_write /\
+        client_after1.CS.model_record.CS.record_read ==
+          R.next_seq client_after0.CS.model_record.CS.record_read /\
+        CS.step_model server_after1 (CS.ConnLocalEvent server_auth_skip) ==
+          Some server_after_auth_skip /\
+        CS.step_model client_after1 (CS.ConnLocalEvent client_auth_skip) ==
+          Some client_after_auth_skip /\
+        CS.step_model
+          server_after_auth_skip
+          (CS.ConnNetworkEvent {
+            CL.message_direction = CL.Sent;
+            CL.message_value = M.TlsHandshake sent_msg2;
+          }) == Some server_after2 /\
+        CS.step_model
+          client_after_auth_skip
+          (CS.ConnNetworkEvent {
+            CL.message_direction = CL.Received;
+            CL.message_value = M.TlsHandshake received_msg2;
+          }) == Some client_after2 /\
+        server_after2.CS.model_record.CS.record_write ==
+          R.next_seq server_after_auth_skip.CS.model_record.CS.record_write /\
+        client_after2.CS.model_record.CS.record_read ==
+          R.next_seq client_after_auth_skip.CS.model_record.CS.record_read /\
+        CS.step_model client_after2 (CS.ConnLocalEvent client_verify_skip) ==
+          Some client_after_verify_skip /\
+        CS.step_model
+          server_after2
+          (CS.ConnNetworkEvent {
+            CL.message_direction = CL.Sent;
+            CL.message_value = M.TlsHandshake sent_msg3;
+          }) == Some server_after3 /\
+        CS.step_model
+          client_after_verify_skip
+          (CS.ConnNetworkEvent {
+            CL.message_direction = CL.Received;
+            CL.message_value = M.TlsHandshake received_msg3;
+          }) == Some client_after3 /\
+        server_after3.CS.model_record.CS.record_write ==
+          R.next_seq server_after2.CS.model_record.CS.record_write /\
+        client_after3.CS.model_record.CS.record_read ==
+          R.next_seq client_after_verify_skip.CS.model_record.CS.record_read /\
+        CS.conn_events_sent_seal_replay
+          server_flight_sender
+          (CS.ConnLocalEvent
+            (CS.LocalInstallTrafficKeysForRole {
+              CS.install_role = CS.ServerEndpoint;
+              CS.install_payload = {
+                CS.install_epoch = CS.TrafficHandshake;
+                CS.install_direction = CS.TrafficWrite;
+                CS.install_material = server_material;
+              };
+            }) :: CS.ConnNetworkEvent {
+              CL.message_direction = CL.Sent;
+              CL.message_value = M.TlsHandshake sent_msg0;
+            } :: CS.ConnNetworkEvent {
+              CL.message_direction = CL.Sent;
+              CL.message_value = M.TlsHandshake sent_msg1;
+            } :: CS.ConnLocalEvent server_auth_skip :: CS.ConnNetworkEvent {
+              CL.message_direction = CL.Sent;
+              CL.message_value = M.TlsHandshake sent_msg2;
+            } :: CS.ConnNetworkEvent {
+              CL.message_direction = CL.Sent;
+              CL.message_value = M.TlsHandshake sent_msg3;
+            } :: server_rest)
+          server_raw_sent
+          server_raw_received
+          server_final /\
+        CS.conn_events_received_decode_replay
+          server_flight_receiver
+          (CS.ConnLocalEvent
+            (CS.LocalInstallTrafficKeys {
+              CS.install_epoch = CS.TrafficHandshake;
+              CS.install_direction = CS.TrafficRead;
+              CS.install_material = client_material;
+            }) :: CS.ConnNetworkEvent {
+              CL.message_direction = CL.Received;
+              CL.message_value = M.TlsHandshake received_msg0;
+            } :: CS.ConnNetworkEvent {
+              CL.message_direction = CL.Received;
+              CL.message_value = M.TlsHandshake received_msg1;
+            } :: CS.ConnLocalEvent client_auth_skip :: CS.ConnNetworkEvent {
+              CL.message_direction = CL.Received;
+              CL.message_value = M.TlsHandshake received_msg2;
+            } :: CS.ConnLocalEvent client_verify_skip :: CS.ConnNetworkEvent {
+              CL.message_direction = CL.Received;
+              CL.message_value = M.TlsHandshake received_msg3;
+            } :: client_rest)
+          client_raw_sent
+          client_raw_received
+          client_final /\
+        write_read_record_material_aligned
+          client_finished_sender
+          client_finished_receiver /\
+        Seq.equal client_finished_raw_sent server_finished_raw_received /\
+        protected_handshake_wire_round_trip_message sent_msg4 /\
+        protected_handshake_wire_round_trip_message received_msg4 /\
+        CS.step_model
+          client_finished_sender
+          (CS.ConnLocalEvent (CS.LocalVerifyFinished verified_server_finished)) ==
+          Some cf_client_after_verify /\
+        CS.step_model
+          cf_client_after_verify
+          (CS.ConnLocalEvent
+            (CS.LocalInstallTrafficKeys {
+              CS.install_epoch = CS.TrafficApplication;
+              CS.install_direction = CS.TrafficWrite;
+              CS.install_material = client_app_write_material;
+            })) == Some cf_client_after_app_write /\
+        CS.step_model
+          cf_client_after_app_write
+          (CS.ConnLocalEvent
+            (CS.LocalInstallTrafficKeys {
+              CS.install_epoch = CS.TrafficApplication;
+              CS.install_direction = CS.TrafficRead;
+              CS.install_material = client_app_read_material;
+            })) == Some cf_client_after_app_read /\
+        CS.step_model
+          client_finished_receiver
+          (CS.ConnLocalEvent
+            (CS.LocalInstallTrafficKeysForRole {
+              CS.install_role = CS.ServerEndpoint;
+              CS.install_payload = {
+                CS.install_epoch = CS.TrafficApplication;
+                CS.install_direction = CS.TrafficWrite;
+                CS.install_material = server_app_write_material;
+              };
+            })) == Some cf_server_after_app_write /\
+        CS.step_model
+          cf_client_after_app_read
+          (CS.ConnNetworkEvent {
+            CL.message_direction = CL.Sent;
+            CL.message_value = M.TlsHandshake sent_msg4;
+          }) == Some cf_client_after_finished /\
+        CS.step_model
+          cf_server_after_app_write
+          (CS.ConnNetworkEvent {
+            CL.message_direction = CL.Received;
+            CL.message_value = M.TlsHandshake received_msg4;
+          }) == Some cf_server_after_finished /\
+        CS.conn_events_sent_seal_replay
+          client_finished_sender
+          (CS.ConnLocalEvent (CS.LocalVerifyFinished verified_server_finished) ::
+           CS.ConnLocalEvent
+             (CS.LocalInstallTrafficKeys {
+               CS.install_epoch = CS.TrafficApplication;
+               CS.install_direction = CS.TrafficWrite;
+               CS.install_material = client_app_write_material;
+             }) ::
+           CS.ConnLocalEvent
+             (CS.LocalInstallTrafficKeys {
+               CS.install_epoch = CS.TrafficApplication;
+               CS.install_direction = CS.TrafficRead;
+               CS.install_material = client_app_read_material;
+             }) ::
+           CS.ConnNetworkEvent {
+             CL.message_direction = CL.Sent;
+             CL.message_value = M.TlsHandshake sent_msg4;
+           } :: client_finished_rest)
+          client_finished_raw_sent
+          client_finished_raw_received
+          client_finished_final /\
+        CS.conn_events_received_decode_replay
+          client_finished_receiver
+          (CS.ConnLocalEvent
+             (CS.LocalInstallTrafficKeysForRole {
+               CS.install_role = CS.ServerEndpoint;
+               CS.install_payload = {
+                 CS.install_epoch = CS.TrafficApplication;
+                 CS.install_direction = CS.TrafficWrite;
+                 CS.install_material = server_app_write_material;
+               };
+             }) ::
+           CS.ConnNetworkEvent {
+             CL.message_direction = CL.Received;
+             CL.message_value = M.TlsHandshake received_msg4;
+           } :: server_finished_rest)
+          server_finished_raw_sent
+          server_finished_raw_received
+          server_finished_final)
+      (ensures
+        exists server_ee server_cert server_cv server_finished client_finished.
+          paired_protected_handshake_event_projection_pairs
+            client_state
+            server_state
+            server_ee
+            server_cert
+            server_cv
+            server_finished
+            client_finished)
+
 val lemma_protected_handshake_event_projection_pair_after_sender_received_network_head
   (sender:CS.connection_model)
   (receiver:CS.connection_model)
